concurrency/HybridMachine_simulation_proof.v
@@ -1,0 +1,377 @@
+Require Import Coq.omega.Omega.
+Require Import Clight.
+Require Import Memory.
+Require Import Values.
+
+Require Import msl.Coqlib2.
+
+Require veric.Clight_core. Import Clight_core.
+
+Require Import concurrency.Smallstep.
+Require Import concurrency.x86_context.
+Require Import concurrency.HybridMachine_simulation.
+Require Import concurrency.compiler_correct.
+Require Import concurrency.CoreSemantics_sum.
+
+Section Clight_Sem.
+  Variable p: program.
+  
+  Notation genv:=genv. (*from Clight_core*)
+  Notation state:=CC_core.
+  
+  Program Definition Clight_memSem: semantics.MemSem genv state:=
+    semantics.Build_MemSem _ _ cl_core_sem _.
+  Next Obligation.
+  Admitted.
+
+  Program Definition Clight_EvSem: event_semantics.EvSem:=
+    event_semantics.Build_EvSem _ _ Clight_memSem _ _ _ _ _.
+  Next Obligation.
+  Admitted.
+  Next Obligation.
+  Admitted.
+  Next Obligation.
+  Admitted.
+  Next Obligation.
+  Admitted.
+  Next Obligation.
+  Admitted.
+    
+  Definition Clight: Semantics_rec:=
+    Build_Semantics_rec
+      genv (*semG*)
+      state (*semC*)
+      Clight_EvSem (*semSem EvSem*).
+End Clight_Sem.
+
+
+Section HybridStepProof.
+
+  Variable p: program.
+  Variable tp: Asm.program. 
+  Variable compiled: (simpl_transf_clight_program p = Errors.OK tp).
+
+  (*Lemma programs_match : simpl_match_prog p tp.
+  Proof. apply transf_clight_program_match; assumption. Qed.
+
+  Lemma program_forward_sim:
+    Smallstep.forward_simulation (semantics2 p) (Asm.semantics tp).
+  Proof. apply simpl_clight_semantic_preservation; apply programs_match; eauto. Qed. *)
+
+  Parameter Clight_step: Clight.genv -> CC_core * mem -> Events.trace -> CC_core * mem -> Prop.
+  Parameter Clight_init: CC_core * mem -> Prop.
+  Parameter Clight_final: CC_core * mem -> Integers.Int.int -> Prop.
+  Parameter Clight_genv: program -> Clight.genv.
+  Parameter Clight_symbolenv: Globalenvs.Senv.t.
+  Definition Clight_semantics2 (p: program) : semantics:=
+    @Semantics_gen
+      CC_core
+      Clight.genv
+      Clight_step
+      Clight_init
+      Clight_final
+      (Clight_genv p)
+      Clight_symbolenv.
+
+  Notation ASM_core:=X86Machines.ErasedMachine.ThreadPool.code.
+  Parameter Asm_step: X86SEM.G -> ASM_core * mem -> Events.trace -> ASM_core * mem -> Prop.
+  Parameter Asm_init: ASM_core * mem -> Prop.
+  Parameter Asm_final: ASM_core * mem -> Integers.Int.int -> Prop.
+  Parameter Asm_genv: Asm.program -> X86SEM.G.
+  Parameter Asm_symbolenv: Globalenvs.Senv.t.
+  Definition Asm_semantics (tp: Asm.program) : semantics:=
+    @Semantics_gen
+      X86Machines.ErasedMachine.ThreadPool.code
+      X86SEM.G
+      Asm_step
+      Asm_init
+      Asm_final
+      (Asm_genv tp)
+      Asm_symbolenv.
+
+  
+  Lemma program_forward_sim:
+    Smallstep.forward_simulation (Clight_semantics2 p) (Asm_semantics tp).
+  Proof. Admitted.
+  
+  Lemma program_forward_properties:
+    exists (index : Type) (order : index -> index -> Prop)
+      (match_states : index -> meminj -> state (Clight_semantics2 p) * mem -> state (Asm_semantics tp) * mem -> Prop
+                        ),
+                         Smallstep.fsim_properties (Clight_semantics2 p) (Asm_semantics tp) index order match_states .
+  Proof. pose proof program_forward_sim as HH.
+         inversion HH. exists index, order, match_states; eauto.
+  Qed.
+
+  Definition Sems:= Clight p.
+  Definition Semt:= X86SEM_rec.  (*How do I pass p to this?*)
+  
+  Variable hb': nat. (*The hybrid bound!*)
+  Definition hb1:= Some hb'.
+  Definition hb2:= Some (S hb').
+
+  Variable U: seq.seq nat. (*The schedule*)
+
+  Notation C1:= (t_ (HybridMachine.ThreadPool hb1 Sems Semt)).
+  Notation C2:= (t_ (HybridMachine.ThreadPool hb2 Sems Semt)).
+  Notation G1:= (semG (HybridMachine.Sem hb1 Sems Semt)) .
+  Notation G2:= (semG (HybridMachine.Sem hb2 Sems Semt)).
+
+  (*The two following globals must be taken from the program...*)
+  (*and they are probaly the smae global??? *)
+  Variable genv: (semG Sems * semG Semt)%type.
+
+
+  (*What are these!!!*)
+  Variable (ge_inv: G1 -> G2 -> Prop).
+  Variable init_inv : meminj -> G1 -> list val -> mem -> G2 -> list val -> mem -> Prop.
+  Variable halt_inv : (*SM_Injection*)meminj -> G1 -> val -> mem -> G2 -> val -> mem -> Prop.
+
+  (* Variable core_ord_wf : well_founded core_ord.
+  Variable thread_match : core_data -> (*SM_Injection*)meminj -> (semC Sems) -> mem -> (semC Semt) -> mem -> Prop. *)
+
+  Definition list_order {A:Type} (order: A -> A -> Prop): list A -> list A -> Prop.
+  Admitted.
+  Lemma list_order_wf: forall {A} ord, @well_founded A ord -> well_founded (list_order ord).
+  Admitted.
+
+  (*Definition list_match
+             {index}
+            (match_states : index -> meminj ->
+                            state (Clight_semantics2 p) * mem ->
+                            state (Asm_semantics tp) * mem -> Prop)
+    (match_source : meminj ->
+                            state (Clight_semantics2 p) -> mem ->
+                            state (Clight_semantics2 p) -> mem -> Prop)
+    (match_target : meminj ->
+                            state (Asm_semantics tp) -> mem ->
+                            state (Asm_semantics tp) -> mem -> Prop):
+    list index -> meminj -> semC Sems -> mem -> semC Semt -> mem -> Prop.
+  (*  |LIST_MATCH: forall lsi j  correct_type: *)
+  Admitted. *)
+
+  Context (match_source : meminj ->
+                            state (Clight_semantics2 p) -> mem ->
+                            state (Clight_semantics2 p) -> mem -> Prop)
+    (match_target : meminj ->
+                            state (Asm_semantics tp) -> mem ->
+                            state (Asm_semantics tp) -> mem -> Prop).
+  
+  Lemma step_hybrid_simulation:
+    exists (core_data: Type), exists (core_ord : core_data -> core_data -> Prop),
+        exists thread_match, exists v:val,
+    HybridMachine_simulation Sems Semt hb1 hb2 U genv ge_inv init_inv halt_inv
+  core_data core_ord thread_match match_source match_target v.  
+  pose proof program_forward_sim as HH.
+  inversion HH.
+  exists (index).
+  exists (order).
+  exists (fun ls mu c1 m1 c2 m2 => match_states ls mu (c1,m1) (c2,m2)).
+  exists Vundef. (*THIS SHOULD DISAPEAR*)
+  constructor.
+  - (*ge_inv*)
+    admit.
+  - (* core_initial*)
+    (* intros.
+    simpl in H.
+    destruct (
+        HybridMachine.init_mach hb1 Sems Semt (@None (prod permissions.access_map permissions.access_map))
+            genv Vundef vals1
+      ) eqn:INIT; 
+    unfold HybridMachine.init_machine' in H;
+    rewrite INIT in H; inversion H; subst. (*solves one case*)
+    unfold HybridMachine.init_mach in INIT.  *)
+    admit.
+  - (*thread_diagram*)
+    intros.
+    destruct U0; simpl in H.
+    + inversion H; subst.
+      inversion HschedN.
+    + inversion H; subst.
+      inversion HschedN; subst.
+      destruct (Compare_dec.lt_eq_lt_dec (S tid) hb') as [[LT | EQ] | LT ].
+      * (*S tid < hb'*)
+      (*This case it's all in source*)
+        inversion Htstep. subst tp' m' ev0.
+        eapply event_semantics.ev_step_ax1 in Hcorestep.
+        unfold hb1 in *.
+        simpl in Hcorestep.
+        simpl in Hcode.
+        assert (Hcode':=Hcode).
+        assert (cnti2:= contains12 _ _ _ _ _ _ _ _ _ _ _ _ _ _ H0 _ Htid).
+        assert (HHH:= Krun_correct_type_source1  _ _ _ _ _ _ _ _ _ _ _ _ _ _
+                                                 H0 _ Htid c).
+        eapply HHH in Hcode'.
+        2: eapply NPeano.Nat.ltb_lt; omega.
+        destruct Hcode' as [c_ Hcode'].
+        subst c; clear HHH.
+
+        
+        assert (TOPROVE: exists c2_, getThreadC cnti2 =
+                                Krun (SState (semC Sems) (semC Semt) c2_)).
+        { eapply correct_type_source1.
+        destruct TOPROVE as [c2_ Hcode2].
+        eapply mtch_source in H0; eauto.
+        
+        
+        (*
+        Unfocus.
+        destruct Hcode as [Hcode c0]; subst c.
+        inversion Hcorestep. subst g s m c' m'.
+        destruct H3 as [NotAtExt step].*)
+        admit.
+
+        
+      * (* S tid = hb' *)
+        (* equal: one machine in source one in target!!*)
+        inversion Htstep. subst tp' m' ev0.
+        eapply event_semantics.ev_step_ax1 in Hcorestep.
+        unfold hb1 in *.
+        simpl in Hcorestep.
+        assert (Hcode':= Hcode).
+        eapply Hinv in Hcode.
+        Focus 2.
+        { subst hb'. eapply NPeano.Nat.ltb_lt; omega. }
+        Unfocus.
+        destruct Hcode as [Hcode c0]; subst c.
+        inversion Hcorestep. subst g s m c' m'.
+        destruct H3 as [NotAtExt step].
+        assert (TOPROVE: forall ge c m t c' m',
+                   Clight.step ge (function_entry2 ge) (CC_core_to_CC_state c m) t (CC_core_to_CC_state c' m') ->
+                    Smallstep.step
+                     (Clight_semantics2 p)
+                     ge (c, m) t (c',m')) by admit.
+        apply TOPROVE in step.
+        assert (TOPROVE2: fst genv = ((globalenv (Clight_semantics2 p)))) by admit.
+        simpl in TOPROVE2.
+        rewrite TOPROVE2 in step.
+        eapply props in step.
+        Focus 2. admit. (*previous match. This follows from concur match *)
+
+        destruct step as [i[[s2' m2'] [mu' [STEP' MATCH]]]].
+        assert (TOPROVE3: containsThread_ (HybridMachine.ThreadPool hb2 Sems Semt) st2 tid) by admit.
+        simpl in Htp'.
+        exists (@updThread_ _ _ _ _ st2 TOPROVE3
+                       (Krun (TState CC_core X86Machines.ErasedMachine.ThreadPool.code  s2'))
+                      (permissions.getCurPerm m2',
+                       snd (getThreadR TOPROVE3))).
+        exists m2'.
+        exists cd. (*This should be updated with the new value!*)
+        exists mu'.
+        split.
+        
+        { (*THE match relation*)
+          clear STEP'.
+          subst st1'; constructor.
+          - simpl. apply H0.
+          - intros.
+            destruct (NPeano.Nat.eq_dec tid i0).
+            + subst i0.
+              admit. (*wrong type of states*)
+            + erewrite gsoThreadCode in H1; auto.
+              simpl in cnti2.
+              unfold updThread_ in H3.
+              erewrite gsoThreadCode in H3; auto.
+              simpl.
+              unfold HybridMachine.compat_th.
+              Parameter same_visible:
+                mem -> mem -> Prop.
+              destruct H0.
+              Lemma match_source_forward:
+                forall mu c1 m1 c2 m2,
+                  match_source mu c1 m1 c2 m2 ->
+                  forall mu' m1' m2',
+                    inject_incr mu mu' ->
+                    same_visible m1 m1' ->
+                    same_visible m2 m2' ->
+                    match_source mu' c1 m1' c2 m2'.
+              Admitted.
+              eapply match_source_forward.
+              * eapply mtch_source; eauto.  
+               admit. (* should be provided by the fsim (compcert simulation)*)
+              * admit. (* should follwo from some combination of memsem steps. *)
+              * admit. (* should follwo from some combination of memsem steps. *)
+          - intros.
+            destruct (NPeano.Nat.eq_dec tid i0).
+            + subst i0.
+              admit. (*wrong type of states*)
+            + erewrite gsoThreadCode in H1; auto.
+              simpl in cnti2.
+              unfold updThread_ in H3.
+              erewrite gsoThreadCode in H3; auto.
+              simpl.
+              unfold HybridMachine.compat_th.
+              destruct H0.
+              Lemma match_target_forward:
+                forall mu c1 m1 c2 m2,
+                  match_target mu c1 m1 c2 m2 ->
+                  forall mu' m1' m2',
+                    inject_incr mu mu' ->
+                    same_visible m1 m1' ->
+                    same_visible m2 m2' ->
+                    match_target mu' c1 m1' c2 m2'.
+              Admitted.
+              eapply match_target_forward.
+              * eapply mtch_target; eauto.  
+               admit. (* should be provided by the fsim (compcert simulation)*)
+              * admit. (* should follwo from some combination of memsem steps. *)
+              * admit. (* should follwo from some combination of memsem steps. *)
+          - intros.
+            destruct (NPeano.Nat.eq_dec tid i0).
+            + subst tid.
+              admit. (*Follows directly from MATCH and the correct update to the list of data*)
+            + admit. (*wrong type of states*)
+           
+        }
+        { (*THE MACHINE STEP.*)
+          admit. (*This should be standard.*)
+        }
+
+      * (* S tid <> hb' ... homogeneous thread is running *)
+        inversion Htstep. subst tp' m' ev0.
+        eapply event_semantics.ev_step_ax1 in Hcorestep.
+        unfold hb1 in *.
+        simpl in Hcorestep.
+        assert (Hcode':= Hcode).
+        eapply Hinv in Hcode.
+        
+        Focus 2.
+        { rewrite <- e; simpl.
+          clear. induction tid; auto. }
+        Unfocus.
+        destruct Hcode as [Hcode c0]; subst c.
+        inversion Hcorestep. subst g s m c' m'.
+        destruct H3 as [NotAtExt step].
+        assert (TOPROVE: forall ge c m t c' m',
+                   Clight.step ge (function_entry2 ge) (CC_core_to_CC_state c m) t (CC_core_to_CC_state c' m') ->
+                    Smallstep.step
+                     (Clight_semantics2 p)
+                     ge (c, m) t (c',m')) by admit.
+        apply TOPROVE in step.
+        assert (TOPROVE2: fst genv = ((globalenv (Clight_semantics2 p)))) by admit.
+        simpl in TOPROVE2.
+        rewrite TOPROVE2 in step.
+        eapply props in step.
+        Focus 2. admit. (*previous match. This follows from concur match *)
+
+        destruct step as [i[[s2' m2'] [mu' [STEP' MATCH]]]].
+        assert (TOPROVE3: containsThread_ (HybridMachine.ThreadPool hb2 Sems Semt) st2 tid) by admit.
+        simpl in Htp'.
+        exists (@updThread_ _ _ _ _ st2 TOPROVE3
+                       (Krun (TState CC_core X86Machines.ErasedMachine.ThreadPool.code  s2'))
+                      (permissions.getCurPerm m2',
+                       snd (getThreadR TOPROVE3))).
+        
+        
+        unfold Step in fsim_simulation.
+        eapply fsim_simulation in step.
+        eapply props0 in step.
+        eapply HH in step.
+        
+
+        
+      * (*not equal: uncompiled thread is running!!*)
+        admit. (*Use an injection mem_sem argumetn*)
+        
+      
+    
