concurrency/self_simulation.v
@@ -1,0 +1,180 @@
+Require Import Coq.omega.Omega.
+Require Import Clight.
+Require Import Memory.
+Require Import Values.
+Require Import Coqlib.
+
+Require Import msl.Coqlib2.
+
+Require veric.Clight_core. Import Clight_core.
+
+Require Import sepcomp.event_semantics.
+Require Import sepcomp.semantics.
+Require Import sepcomp.mem_lemmas.
+
+
+Require Import concurrency.Smallstep.
+Require Import concurrency.x86_context.
+Require Import concurrency.HybridMachine_simulation.
+Require Import concurrency.compiler_correct.
+Require Import concurrency.CoreSemantics_sum.
+
+
+(*Self simulations say that a program has equivalent executions 
+  in equivalent memories. 
+  - Equivalent memories: VISIBLE locations are injected 
+    one to one (same values and permissions).
+  - Equivalent executions: the executions have equivalent memories and
+    none visible locations are unchanged (in the execution).  
+*)
+Section SelfSim.
+
+  Parameter G C: Type.
+  Parameter Sem: MemSem G C.
+
+  (*extension of a mem_injection*)
+  Definition is_ext (f1:meminj)(nb1: positive)(f2:meminj)(nb2:positive) : Prop:=
+    forall b1 b2 ofs,
+      f2 b1 = Some (b2, ofs) ->
+      f1 b1 = Some (b2, ofs) /\
+      (ofs = 0 /\ ~ Plt b1 nb1 /\  ~ Plt b2 nb2).
+  
+  (*The code is also injected*)
+  Parameter code_inject: C -> meminj -> C -> Prop.
+  Parameter code_inj_incr: forall c1 mu c2 mu',
+      code_inject c1 mu c2 ->
+      inject_incr mu mu' ->
+      code_inject c1 mu' c2.
+  
+  (*The current permisions OF THIS THREAD are unchanged! *)
+  (*This is slightly stronger than Mem.inject/mi_inj which allows
+    permissions to grow (on compilation). *)
+  (*also it could be restricted to take only the Cur permissions*)
+  Definition perm_inject (f:meminj)(m1:mem)(m2:mem): Prop:=
+    forall b1 b2 delta,
+      f b1 = Some (b2, delta) ->
+      forall ofs p,
+        Mem.perm m1 b1 (ofs ) Cur p  <->
+        Mem.perm m2 b2 (ofs + delta) Cur p.
+
+  (* The injection maps all visible locations*)
+  Definition perm_image (f:meminj)(m1:mem)(m2:mem): Prop:=
+    forall b1 ofs,
+      Mem.perm m1 b1 ofs Cur Nonempty ->
+    exists b2 delta,
+      f b1 = Some (b2, delta).
+
+  (* The injection maps to every visible location *)
+  Definition perm_preimage (f:meminj)(m1:mem)(m2:mem): Prop:=
+    forall b2 ofs_delta,
+      Mem.perm m2 b2 ofs_delta Cur Nonempty ->
+    exists b1 delta ofs,
+      f b1 = Some (b2, delta) /\
+      Mem.perm m1 b1 ofs Cur Nonempty /\
+  ofs_delta = ofs + delta. 
+  
+  (*TODO: fill in*)
+  Record match_self (f: meminj) (c1:C) (m1:mem) (c2:C) (m2:mem): Prop:=
+    { cinject: code_inject c1 f c2
+    ; minject: Mem.inject f m1 m2            
+    ; pinject: perm_inject f m1 m2
+    ; pimage: perm_image f m1 m2
+    ; ppreimage: perm_preimage f m1 m2
+    }.
+
+  Record same_visible (m1 m2: mem):=
+    { same_visible12:
+        forall b ofs,
+          Mem.perm m1 b ofs Cur Nonempty ->
+          (forall p, Mem.perm m1 b ofs Cur p <->
+                Mem.perm m2 b ofs Cur p) /\
+          (Maps.ZMap.get ofs (Maps.PMap.get b (Mem.mem_contents m1))) =
+          (Maps.ZMap.get ofs (Maps.PMap.get b (Mem.mem_contents m2)));
+      same_visible21:
+        forall b ofs,
+          Mem.perm m2 b ofs Cur Nonempty ->
+          (forall p, Mem.perm m1 b ofs Cur p <->
+                Mem.perm m2 b ofs Cur p) /\
+          (Maps.ZMap.get ofs (Maps.PMap.get b (Mem.mem_contents m1))) =
+          (Maps.ZMap.get ofs (Maps.PMap.get b (Mem.mem_contents m2)));
+      }.
+            
+  Lemma match_source_forward:
+    forall mu c1 m1 c2 m2,
+      match_self mu c1 m1 c2 m2 ->
+      forall mu' m1' m2',
+        inject_incr mu mu' ->
+        Mem.inject mu' m1' m2' ->
+        same_visible m1 m1' ->
+        same_visible m2 m2' ->
+        match_self mu' c1 m1' c2 m2'.
+  Proof.
+    intros. constructor.
+    - eapply code_inj_incr; eauto. eapply H.
+    - assumption.
+    - unfold perm_inject; intros.
+      inversion H.
+      simpl; split; intros.
+      + assert (NE: Mem.perm m1' b1 ofs Cur Nonempty)
+          by admit. (*easy by transitivity that doenst' exists*)
+        assert (NE':= NE).
+        eapply same_visible21 in NE'; eauto.
+        destruct NE' as [SAME_PERM SAME_CONTENT].
+        apply SAME_PERM in H5.
+        apply SAME_PERM in NE.
+        eapply H in H5.
+
+        eapply same_visible12 with (m2:=m2') in H5; eauto.
+        admit. (*by trans *)
+        
+        eapply pimage0 in NE.
+        destruct NE as [? [? HH]].
+        assert (HH':= HH).
+        eapply H0 in HH'.
+        rewrite HH' in H4; inversion H4; subst.
+        assumption.
+      + assert (NE: Mem.perm m2' b2 (ofs+delta) Cur Nonempty)
+          by admit. (*easy by transitivity that doenst' exists*)
+        assert (NE':= NE).
+        eapply same_visible21 in NE'; eauto.
+        destruct NE' as [SAME_PERM SAME_CONTENT].
+        apply SAME_PERM in H5.
+        apply SAME_PERM in NE.
+        eapply pinject0 in H5.
+        
+        eapply same_visible12 with (m2:=m1') in H5; eauto.
+        admit. (*by trans *)
+        
+        eapply ppreimage0 in NE.
+        destruct NE as [? [? [? [HH1 [HH2 HH3]]]]].
+        assert (HH':= HH1).
+        eapply H0 in HH'.
+        admit. (*With some none overlapping this should follow*)
+    - (*pre_image*)
+      intros b1 ofs PERM.
+      admit. (*Easy ... use lemmas to simplify same_visible*)
+    - intros b2 ofs_delta PERM.
+      admit. (*Easy ... use lemmas to simplify same_visible*)
+  Admitted.
+
+  Record self_simulation :Prop :=
+    { ssim_diagram: forall f c1 m1 c2 m2,
+        match_self f c1 m1 c2 m2 ->
+        forall g c1' m1',
+          corestep Sem g c1 m1 c1' m1' ->
+          exists c2' m2' f',
+          corestep Sem g c2 m2 c2' m2' /\
+          match_self f c1' m1' c2' m2' /\
+          is_ext f (Mem.nextblock m1) f' (Mem.nextblock m2)        
+    }.
+
+  
+
+End SelfSim.
+
+  
+        
+
+  
+  
+  
